Px86 ptoa: finish fob
Signed-off-by: Kyeongmin Cho <kyeongmin.cho@kaist.ac.kr>

src/axiomatic/TsoSimLocal.v
@@ -417,7 +417,12 @@ Proof.
       eauto 10 using union_l, union_r.
 Qed.
 
+(* CHECK: add flush *)
 Definition sim_local_lper ex loc :=
+  (sim_local_vwn ex ⨾
+   ⦗ex.(Execution.label_is) (Label.is_flushing loc)⦘ ⨾
+   Execution.po) ∪
+
   ((sim_local_coh ex loc ∪ sim_local_vpn ex) ⨾
    ⦗ex.(Execution.label_is) (Label.is_flushopting loc)⦘ ⨾
    Execution.po).
@@ -425,19 +430,29 @@ Definition sim_local_lper ex loc :=
 Lemma sim_local_lper_step ex loc:
   sim_local_lper ex loc =
   (sim_local_lper ex loc ∪
-   ((sim_local_coh ex loc ∪ sim_local_vpn ex) ⨾
-    ⦗ex.(Execution.label_is) (Label.is_flushopting loc)⦘)) ⨾
+   ((sim_local_vwn ex ⨾
+     ⦗ex.(Execution.label_is) (Label.is_flushing loc)⦘) ∪
+    ((sim_local_coh ex loc ∪ sim_local_vpn ex) ⨾
+     ⦗ex.(Execution.label_is) (Label.is_flushopting loc)⦘))) ⨾
   Execution.po_adj.
 Proof.
   unfold sim_local_lper. rewrite ? (union_seq' Execution.po_adj), ? seq_assoc, ? union_assoc.
-  rewrite Execution.po_po_adj at 1.
+  rewrite Execution.po_po_adj at 1 2.
   rewrite (clos_refl_union Execution.po).
   replace ((Execution.po ∪ eq) ⨾ Execution.po_adj)
     with (Execution.po ⨾ Execution.po_adj ∪ eq ⨾ Execution.po_adj); cycle 1.
   { rewrite union_seq. ss. }
   rewrite eq_seq.
   rewrite ? (seq_union' (Execution.po ⨾ Execution.po_adj) Execution.po_adj), ? seq_assoc, ? union_assoc.
-  refl.
+  funext. i. funext. i. propext. econs; i.
+  - repeat match goal with
+           | [H: (_ ∪ _) _ _ |- _] => inv H
+           end;
+      eauto 10 using union_l, union_r.
+  - repeat match goal with
+           | [H: (_ ∪ _) _ _ |- _] => inv H
+           end;
+      eauto 10 using union_l, union_r.
 Qed.
 
 Definition sim_local_per ex loc :=
@@ -445,9 +460,7 @@ Definition sim_local_per ex loc :=
    ⦗ex.(Execution.label_is) (Label.is_flushing loc)⦘ ⨾
    Execution.po) ∪
 
-  ((sim_local_coh ex loc ∪ sim_local_vpn ex) ⨾
-   ⦗ex.(Execution.label_is) (Label.is_flushopting loc)⦘ ⨾
-   Execution.po ⨾
+  (sim_local_lper ex loc ⨾
    ⦗ex.(Execution.label_is) (Label.is_persist_barrier)⦘ ⨾
    Execution.po).
 
@@ -455,17 +468,15 @@ Lemma sim_local_per_step ex loc:
   sim_local_per ex loc =
   (sim_local_per ex loc ∪
    ((sim_local_vwn ex ⨾
-    ⦗ex.(Execution.label_is) (Label.is_flushing loc)⦘) ∪
+     ⦗ex.(Execution.label_is) (Label.is_flushing loc)⦘) ∪
 
-    ((sim_local_coh ex loc ∪ sim_local_vpn ex) ⨾
-    ⦗ex.(Execution.label_is) (Label.is_flushopting loc)⦘ ⨾
-    Execution.po ⨾
-    ⦗ex.(Execution.label_is) (Label.is_persist_barrier)⦘))) ⨾
+    (sim_local_lper ex loc ⨾
+     ⦗ex.(Execution.label_is) (Label.is_persist_barrier)⦘))) ⨾
   Execution.po_adj.
 Proof.
   unfold sim_local_per.
   rewrite ? (union_seq' Execution.po_adj), ? seq_assoc, ? union_assoc.
-  rewrite Execution.po_po_adj at 1 3.
+  rewrite Execution.po_po_adj at 1 2.
   rewrite (clos_refl_union Execution.po).
   replace ((Execution.po ∪ eq) ⨾ Execution.po_adj)
     with (Execution.po ⨾ Execution.po_adj ∪ eq ⨾ Execution.po_adj); cycle 1.
